VCVio/CryptoFoundations/Fork.lean
@@ -36,28 +36,29 @@ structure forkInput (spec : OracleSpec ι) (α : Type) where
 /-- Version of `fork` that doesn't choose `s` ahead of time.
 Should give better concrete bounds. -/
 def fork' (main : OracleComp spec α) (qb : ι → ℕ)
-    (js : List ι) (i : ι) (cf : α → Option (Fin (qb i))) :
+    (js : List ι) (i : ι) (cf : α → Option (Fin (qb i + 1))) :
     OracleComp spec (α × α) := do
-  let seed : QuerySeed spec ← generateSeed spec qb js
+  let seed ← generateSeed spec qb js
   let x₁ ← (simulateQ seededOracle main).run seed
-  let s : Fin (qb i) ← (cf x₁).getM
+  let s : Fin (qb i + 1) ← (cf x₁).getM
   let u ←$ᵗ spec.range i
-  guard ((seed i)[s]? ≠ some u) -- Didn't pick the same output
+  guard ((seed i)[s + 1]? ≠ some u) -- Didn't pick the same output
   let seed' := (seed.takeAtIndex i s).addValue i u
   let x₂ ← (simulateQ seededOracle main).run seed'
   guard (cf x₂ = some s) -- New output corresponds to the same fork
   return (x₁, x₂)
 
 theorem le_probFailure_fork' (main : OracleComp spec α) (qb : ι → ℕ)
-    (js : List ι) (i : ι) (cf : α → Option (Fin (qb i))) [spec.FiniteRange] :
+    (js : List ι) (i : ι) (cf : α → Option (Fin (qb i + 1))) [spec.FiniteRange] :
     let acc : ℝ≥0∞ := [= none | cf <$> main]
     let h : ℝ≥0∞ := Fintype.card (spec.range i)
     [⊥ | fork' main qb js i cf] ≤ acc * (1 / h + acc / qb i) := by
   rw [fork']
   rw [probFailure_bind_of_neverFails]
-  ·
+  · simp only
     sorry
-  sorry
+  · simp
+    sorry
 
 def fork (main : OracleComp spec α) (i : ι) (qb : ι → ℕ)
     (js : List ι) (cf : α → QueryLog spec → Option (Fin (qb i + 1))) :
